Remove CAS loop in release of ticket_lock.

heap_lang/lib/ticket_lock.v
@@ -1,9 +1,8 @@
 From iris.program_logic Require Export weakestpre.
 From iris.heap_lang Require Export lang.
-From iris.program_logic Require Import auth.
 From iris.proofmode Require Import invariants.
 From iris.heap_lang Require Import proofmode notation.
-From iris.algebra Require Import gset.
+From iris.algebra Require Import auth gset.
 From iris.heap_lang.lib Require Export lock.
 Import uPred.
 
@@ -23,53 +22,44 @@ Definition acquire : val :=
       then wait_loop "n" "lock"
       else "acquire" "lock".
 
-Definition release : val :=
-  rec: "release" "lock" :=
-    let: "o" := !(Fst "lock") in
-    if: CAS (Fst "lock") "o" ("o" + #1)
-      then #()
-      else "release" "lock".
+Definition release : val := λ: "lock",
+  (Fst "lock") <- !(Fst "lock") + #1.
 
 Global Opaque newlock acquire release wait_loop.
 
 (** The CMRAs we need. *)
-Class tlockG Σ := TlockG {
-   tlock_G :> authG Σ (gset_disjUR nat);
-   tlock_exclG  :> inG Σ (exclR unitC)
-}.
+Class tlockG Σ :=
+  tlock_G :> inG Σ (authR (prodUR (optionUR (exclR natC)) (gset_disjUR nat))).
 Definition tlockΣ : gFunctors :=
-  #[authΣ (gset_disjUR nat); GFunctor (constRF (exclR unitC))].
+  #[ GFunctor (constRF (authR (prodUR (optionUR (exclR natC)) (gset_disjUR nat)))) ].
 
 Instance subG_tlockΣ {Σ} : subG tlockΣ Σ → tlockG Σ.
-Proof. intros [? [?%subG_inG _]%subG_inv]%subG_inv. split; apply _. Qed.
+Proof. by intros ?%subG_inG. Qed.
 
 Section proof.
   Context `{!heapG Σ, !tlockG Σ} (N : namespace).
 
-  Definition tickets_inv (n: nat) (gs: gset_disjUR nat) : iProp Σ :=
-    (gs = GSet (seq_set 0 n))%I.
+  Definition lock_inv (γ : gname) (lo ln : loc) (R : iProp Σ) : iProp Σ :=
+    (∃ o n : nat,
+      lo ↦ #o ★ ln ↦ #n ★
+      own γ (● (Excl' o, GSet (seq_set 0 n))) ★
+      ((own γ (◯ (Excl' o, ∅)) ★ R) ∨ own γ (◯ (∅, GSet {[ o ]}))))%I.
 
-  Definition lock_inv (γ1 γ2: gname) (lo ln: loc) (R : iProp Σ) : iProp Σ :=
-    (∃ (o n: nat),
-       lo ↦ #o ★ ln ↦ #n ★
-       auth_inv γ1 (tickets_inv n) ★
-       ((own γ2 (Excl ()) ★ R) ∨ auth_own γ1 (GSet {[ o ]})))%I.
-
-  Definition is_lock (γs: gname * gname) (l: val) (R: iProp Σ) : iProp Σ :=
-    (∃ (lo ln: loc),
+  Definition is_lock (γ : gname) (lk : val) (R : iProp Σ) : iProp Σ :=
+    (∃ lo ln : loc,
        heapN ⊥ N ∧ heap_ctx ∧
-       l = (#lo, #ln)%V ∧ inv N (lock_inv (fst γs) (snd γs) lo ln R))%I.
+       lk = (#lo, #ln)%V ∧ inv N (lock_inv γ lo ln R))%I.
 
-  Definition issued (γs: gname * gname) (l : val) (x: nat) (R : iProp Σ) : iProp Σ :=
-    (∃ (lo ln: loc),
+  Definition issued (γ : gname) (lk : val) (x : nat) (R : iProp Σ) : iProp Σ :=
+    (∃ lo ln: loc,
        heapN ⊥ N ∧ heap_ctx ∧
-       l = (#lo, #ln)%V ∧ inv N (lock_inv (fst γs) (snd γs) lo ln R) ∧
-       auth_own (fst γs) (GSet {[ x ]}))%I.
+       lk = (#lo, #ln)%V ∧ inv N (lock_inv γ lo ln R) ∧
+       own γ (◯ (∅, GSet {[ x ]})))%I.
 
-  Definition locked (γs: gname * gname) : iProp Σ := own (snd γs) (Excl ())%I.
+  Definition locked (γ : gname) : iProp Σ := (∃ o, own γ (◯ (Excl' o, ∅)))%I.
 
-  Global Instance lock_inv_ne n γ1 γ2 lo ln :
-    Proper (dist n ==> dist n) (lock_inv γ1 γ2 lo ln).
+  Global Instance lock_inv_ne n γs lo ln :
+    Proper (dist n ==> dist n) (lock_inv γs lo ln).
   Proof. solve_proper. Qed.
   Global Instance is_lock_ne γs n l : Proper (dist n ==> dist n) (is_lock γs l).
   Proof. solve_proper. Qed.
@@ -78,47 +68,41 @@ Section proof.
   Global Instance locked_timeless γs : TimelessP (locked γs).
   Proof. apply _. Qed.
 
-  Lemma locked_exclusive (γs: gname * gname) : (locked γs ★ locked γs ⊢ False)%I.
-  Proof. rewrite /locked -own_op own_valid. by iIntros (?). Qed.
+  Lemma locked_exclusive (γ : gname) : (locked γ ★ locked γ ⊢ False)%I.
+  Proof.
+    iIntros "[H1 H2]". iDestruct "H1" as (o1) "H1". iDestruct "H2" as (o2) "H2".
+    iCombine "H1" "H2" as "H". iDestruct (own_valid with "H") as %[[] _].
+  Qed.
 
   Lemma newlock_spec (R : iProp Σ) Φ :
     heapN ⊥ N →
-    heap_ctx ★ R ★ (∀ lk γs, is_lock γs lk R -★ Φ lk) ⊢ WP newlock #() {{ Φ }}.
+    heap_ctx ★ R ★ (∀ lk γ, is_lock γ lk R -★ Φ lk) ⊢ WP newlock #() {{ Φ }}.
   Proof.
     iIntros (HN) "(#Hh & HR & HΦ)". rewrite /newlock /=.
     wp_seq. wp_alloc lo as "Hlo". wp_alloc ln as "Hln".
-    iVs (own_alloc (Excl ())) as (γ2) "Hγ2"; first done.
-    iVs (own_alloc_strong (Auth (Excl' ∅) ∅) {[ γ2 ]}) as (γ1) "[% Hγ1]"; first done.
-    iVs (inv_alloc N _ (lock_inv γ1 γ2 lo ln R) with "[-HΦ]").
-    - iNext. rewrite /lock_inv.
-      iExists 0%nat, 0%nat.
-      iFrame.
-      iSplitL "Hγ1".
-      + rewrite /auth_inv.
-        iExists (GSet ∅).
-        by iFrame.
-      + iLeft. by iFrame.
-    - iVsIntro.
-      iApply ("HΦ" $! (#lo, #ln)%V (γ1, γ2)).
-      iExists lo, ln.
-      iSplit; by eauto.
+    iVs (own_alloc (● (Excl' 0%nat, ∅) ⋅ ◯ (Excl' 0%nat, ∅))) as (γ) "[Hγ Hγ']".
+    { by rewrite -auth_both_op. }
+    iVs (inv_alloc _ _ (lock_inv γ lo ln R) with "[-HΦ]").
+    { iNext. rewrite /lock_inv.
+      iExists 0%nat, 0%nat. iFrame. iLeft. by iFrame. }
+    iVsIntro. iApply ("HΦ" $! (#lo, #ln)%V γ). iExists lo, ln. eauto.
   Qed.
 
-  Lemma wait_loop_spec γs l x R (Φ : val → iProp Σ) :
-    issued γs l x R ★ (locked γs -★ R -★ Φ #()) ⊢ WP wait_loop #x l {{ Φ }}.
+  Lemma wait_loop_spec γ l x R (Φ : val → iProp Σ) :
+    issued γ l x R ★ (locked γ -★ R -★ Φ #()) ⊢ WP wait_loop #x l {{ Φ }}.
   Proof.
     iIntros "[Hl HΦ]". iDestruct "Hl" as (lo ln) "(% & #? & % & #? & Ht)".
     iLöb as "IH". wp_rec. subst. wp_let. wp_proj. wp_bind (! _)%E.
-    iInv N as (o n) "[Hlo [Hln Ha]]" "Hclose".
+    iInv N as (o n) "(Hlo & Hln & Ha)" "Hclose".
     wp_load. destruct (decide (x = o)) as [->|Hneq].
     - iDestruct "Ha" as "[Hainv [[Ho HR] | Haown]]".
-      + iVs ("Hclose" with "[Hlo Hln Hainv Ht]").
+      + iVs ("Hclose" with "[Hlo Hln Hainv Ht]") as "_".
         { iNext. iExists o, n. iFrame. eauto. }
         iVsIntro. wp_let. wp_op=>[_|[]] //.
         wp_if. iVsIntro.
-        iApply ("HΦ" with "[-HR] HR"). eauto.
+        iApply ("HΦ" with "[-HR] HR"). rewrite /locked; eauto.
       + iExFalso. iCombine "Ht" "Haown" as "Haown".
-        iDestruct (auth_own_valid with "Haown") as % ?%gset_disj_valid_op.
+        iDestruct (own_valid with "Haown") as % [_ ?%gset_disj_valid_op].
         set_solver.
     - iVs ("Hclose" with "[Hlo Hln Ha]").
       { iNext. iExists o, n. by iFrame. }
@@ -126,64 +110,72 @@ Section proof.
       wp_if. iApply ("IH" with "Ht"). by iExact "HΦ".
   Qed.
 
-  Lemma acquire_spec γs l R (Φ : val → iProp Σ) :
-    is_lock γs l R ★ (locked γs -★ R -★ Φ #()) ⊢ WP acquire l {{ Φ }}.
+  Lemma acquire_spec γ l R (Φ : val → iProp Σ) :
+    is_lock γ l R ★ (locked γ -★ R -★ Φ #()) ⊢ WP acquire l {{ Φ }}.
   Proof.
     iIntros "[Hl HΦ]". iDestruct "Hl" as (lo ln) "(% & #? & % & #?)".
     iLöb as "IH". wp_rec. wp_bind (! _)%E. subst. wp_proj.
     iInv N as (o n) "[Hlo [Hln Ha]]" "Hclose".
-    wp_load. iVs ("Hclose" with "[Hlo Hln Ha]").
+    wp_load. iVs ("Hclose" with "[Hlo Hln Ha]") as "_".
     { iNext. iExists o, n. by iFrame. }
     iVsIntro. wp_let. wp_proj. wp_op.
     wp_bind (CAS _ _ _).
-    iInv N as (o' n') "[Hlo' [Hln' [Hainv Haown]]]" "Hclose".
+    iInv N as (o' n') "(>Hlo' & >Hln' & >Hauth & Haown)" "Hclose".
     destruct (decide (#n' = #n))%V as [[= ->%Nat2Z.inj] | Hneq].
     - wp_cas_suc.
-      iDestruct "Hainv" as (s) "[Ho %]"; subst.
-      iVs (own_update with "Ho") as "Ho".
-      { eapply auth_update_no_frag, (gset_disj_alloc_empty_local_update n).
-        rewrite elem_of_seq_set; omega. }
-      iDestruct "Ho" as "[Hofull Hofrag]".
-      iVs ("Hclose" with "[Hlo' Hln' Haown Hofull]").
-      { rewrite gset_disj_union; last by apply (seq_set_S_disjoint 0).
-        rewrite -(seq_set_S_union_L 0).
-        iNext. iExists o', (S n)%nat.
-        rewrite Nat2Z.inj_succ -Z.add_1_r.
-        iFrame. iExists (GSet (seq_set 0 (S n))). by iFrame. }
+      iVs (own_update with "Hauth") as "Hauth".
+      { eapply (auth_update_no_frag _ (∅, _)), prod_local_update,
+          (gset_disj_alloc_empty_local_update n); [done|].
+        rewrite elem_of_seq_set. omega. }
+      rewrite pair_op left_id_L. iDestruct "Hauth" as "[Hauth Hofull]".
+      rewrite gset_disj_union; last by apply (seq_set_S_disjoint 0).
+      rewrite -(seq_set_S_union_L 0).
+      iVs ("Hclose" with "[Hlo' Hln' Haown Hauth]") as "_".
+      { iNext. iExists o', (S n).
+        rewrite Nat2Z.inj_succ -Z.add_1_r. by iFrame. }
       iVsIntro. wp_if.
-      iApply (wait_loop_spec γs (#lo, #ln)).
-      iSplitR "HΦ"; last by auto.
-      rewrite /issued /auth_own; eauto 10.
+      iApply (wait_loop_spec γ (#lo, #ln)).
+      iFrame "HΦ". rewrite /issued; eauto 10.
     - wp_cas_fail.
-      iVs ("Hclose" with "[Hlo' Hln' Hainv Haown]").
+      iVs ("Hclose" with "[Hlo' Hln' Hauth Haown]").
       { iNext. iExists o', n'. by iFrame. }
       iVsIntro. wp_if. by iApply "IH".
   Qed.
 
-  Lemma release_spec γs l R (Φ : val → iProp Σ):
-    is_lock γs l R ★ locked γs ★ R ★ Φ #() ⊢ WP release l {{ Φ }}.
+  Lemma release_spec γ l R (Φ : val → iProp Σ):
+    is_lock γ l R ★ locked γ ★ R ★ Φ #() ⊢ WP release l {{ Φ }}.
   Proof.
-    iIntros "(Hl & Hγ & HR & HΦ)". iDestruct "Hl" as (lo ln) "(% & #? & % & #?)".
-    iLöb as "IH". wp_rec. subst. wp_proj. wp_bind (! _)%E.
-    iInv N as (o n) "[Hlo [Hln Hr]]" "Hclose".
-    wp_load. iVs ("Hclose" with "[Hlo Hln Hr]").
+    iIntros "(Hl & Hγ & HR & HΦ)".
+    iDestruct "Hl" as (lo ln) "(% & #? & % & #?)"; subst.
+    iDestruct "Hγ" as (o) "Hγo".
+    rewrite /release. wp_let. wp_proj. wp_proj. wp_bind (! _)%E.
+    iInv N as (o' n) "(>Hlo & >Hln & >Hauth & Haown)" "Hclose".
+    wp_load.
+    iAssert (o' = o)%I with "[#]" as "%"; subst.
+    { iCombine "Hγo" "Hauth" as "Hγo".
+      by iDestruct (own_valid with "Hγo") (* FIXME: this is horrible *)
+        as %[[[[?|] ?] [=]%leibniz_equiv_iff] ?]%auth_valid_discrete. }
+    iVs ("Hclose" with "[Hlo Hln Hauth Haown]") as "_".
     { iNext. iExists o, n. by iFrame. }
-    iVsIntro. wp_let. wp_bind (CAS _ _ _ ).
-    wp_proj. wp_op.
-    iInv N as (o' n') "[Hlo' [Hln' Hr]]" "Hclose".
-    destruct (decide (#o' = #o))%V as [[= ->%Nat2Z.inj ] | Hneq].
-    - wp_cas_suc.
-      iDestruct "Hr" as "[Hainv [[Ho _] | Hown]]".
-      + iExFalso. iCombine "Hγ" "Ho" as "Ho".
-        iDestruct (own_valid with "#Ho") as %[].
-      + iVs ("Hclose" with "[Hlo' Hln' HR Hγ Hainv]").
-        { iNext. iExists (o + 1)%nat, n'%nat.
-          iFrame. rewrite Nat2Z.inj_add.
-          iFrame. iLeft; by iFrame. }
-        iVsIntro. by wp_if.
-    - wp_cas_fail. iVs ("Hclose" with "[Hlo' Hln' Hr]").
-      { iNext. iExists o', n'. by iFrame. }
-      iVsIntro. wp_if. by iApply ("IH" with "Hγ HR").
+    iVsIntro. wp_op.
+    iInv N as (o' n') "(>Hlo & >Hln & >Hauth & Haown)" "Hclose".
+    wp_store.
+    iAssert (o' = o)%I with "[#]" as "%"; subst.
+    { iCombine "Hγo" "Hauth" as "Hγo".
+      by iDestruct (own_valid with "Hγo")
+        as %[[[[?|] ?] [=]%leibniz_equiv_iff] ?]%auth_valid_discrete. }
+    iDestruct "Haown" as "[[Hγo' _]|?]".
+    { iCombine "Hγo" "Hγo'" as "Hγo".
+      iDestruct (own_valid with "#Hγo") as %[[] ?]. }
+    iCombine "Hauth" "Hγo" as "Hauth".
+    iVs (own_update with "Hauth") as "Hauth".
+    { rewrite pair_split_L. apply: (auth_update _ _ (Excl' (S o), _)). (* FIXME: apply is slow *)
+      apply prod_local_update, reflexivity; simpl.
+      by apply option_local_update, exclusive_local_update. }
+    rewrite -pair_split_L. iDestruct "Hauth" as "[Hauth Hγo]".
+    iVs ("Hclose" with "[Hlo Hln Hauth Haown Hγo HR]") as "_"; last auto.
+    iNext. iExists (S o), n'.
+    rewrite Nat2Z.inj_succ -Z.add_1_r. iFrame. iLeft. by iFrame.
   Qed.
 End proof.
 
